WIP

bedrock2/src/ImpWithIO.v
@@ -1,4 +1,4 @@
-Require compiler.Common.
+Require compiler.util.Common.
 
 Local Notation "'bind_Some' x <- a ; f" :=
   (match a with
@@ -18,14 +18,14 @@ Class ImpParameters :=
     bopname : Type;
     mem : Type;
 
-    varmap : Type;
-    varmap_operations : Common.Map varmap varname mword;
+    varmap_functions : compiler.util.Map.MapFunctions varname mword;
 
     interp_binop : bopname -> mword -> mword -> mword;
     load : mword -> mem -> option mword;
     store : mword -> mword -> mem -> option mem;
   }.
-Global Existing Instance varmap_operations.
+Global Existing Instance varmap_functions.
+Definition varmap {p:ImpParameters} : Type := Map.map varname mword.
 
 Section Imp.
   Goal True. let cls := constr:(ImpParameters) in match constr:(Set) with _ => (let none := constr:(_:cls) in idtac); fail 99 "DUPLICATE INSTANCE" | _ => idtac end. Abort.
@@ -61,92 +61,92 @@ Section Imp.
   Definition BStack (caller_locals : varmap) (callee : blocked) (binds rets: list varname) : blocked :=
     fun values => bind_Some (callee_locals, c) <- callee values; Some (caller_locals, CStack callee_locals c binds rets).
 
-  Fixpoint interp_expr (st:varmap) (e:expr) : option mword :=
+  Fixpoint interp_expr (l:varmap) (e:expr) : option mword :=
     match e with
     | ELit v => Some v
-    | EVar x => Common.get st x
+    | EVar x => Map.get l x
     | EOp op e1 e2 =>
-      bind_Some v1 <- interp_expr st e1;
-        bind_Some v2 <- interp_expr st e2;
+      bind_Some v1 <- interp_expr l e1;
+        bind_Some v2 <- interp_expr l e2;
         Some (interp_binop op v1 v2)
     end.
 
   Definition computation_result : Type := mem * (actname * list mword * blocked + varmap).
   Section WithFunctions.
     Context (lookupFunction : funname -> option (list varname * list varname * stmt)).
-    Fixpoint interp_stmt(f: nat)(st: varmap)(m: mem)(s: stmt): option computation_result :=
+    Fixpoint interp_stmt(f: nat)(m: mem)(l: varmap)(s: stmt): option computation_result :=
       match f with
       | 0 => None (* out of fuel *)
       | S f => match s with
         | SLoad x a =>
-          bind_Some a <- interp_expr st a;
+          bind_Some a <- interp_expr l a;
           bind_Some v <- load a m;
-          Some (m, inr (Common.put st x v))
+          Some (m, inr (Map.put l x v))
         | SStore a v =>
-          bind_Some a <- interp_expr st a;
-          bind_Some v <- interp_expr st v;
+          bind_Some a <- interp_expr l a;
+          bind_Some v <- interp_expr l v;
           bind_Some m <- store a v m;
-          Some (m, inr st)
+          Some (m, inr l)
         | SSet x e =>
-          bind_Some v <- interp_expr st e;
-          Some (m, inr (Common.put st x v))
+          bind_Some v <- interp_expr l e;
+          Some (m, inr (Map.put l x v))
         | SIf cond bThen bElse =>
-          bind_Some v <- interp_expr st cond;
-          interp_stmt f st m (if mword_nonzero v then bThen else bElse)
+          bind_Some v <- interp_expr l cond;
+          interp_stmt f m l (if mword_nonzero v then bThen else bElse)
         | SWhile cond body =>
-          bind_Some v <- interp_expr st cond;
+          bind_Some v <- interp_expr l cond;
           if mword_nonzero v
           then
-            bind_Some (m, ob) <- interp_stmt f st m body;
+            bind_Some (m, ob) <- interp_stmt f m l body;
             match ob with
             | inl (action, args, b) => Some (m, inl (action, args, BSeq b (SWhile cond body)))
-            | inr st => interp_stmt f st m (SWhile cond body)
+            | inr l => interp_stmt f m l (SWhile cond body)
             end
-          else Some (m, inr st)
+          else Some (m, inr l)
         | SSeq s1 s2 =>
-          bind_Some (m, ob) <- interp_stmt f st m s1;
+          bind_Some (m, ob) <- interp_stmt f m l s1;
           match ob with
           | inl (action, args, b) => Some (m, inl (action, args, BSeq b s2))
-          | inr st => interp_stmt f st m s2
+          | inr l => interp_stmt f m l s2
           end
-        | SSkip => Some (m, inr st)
+        | SSkip => Some (m, inr l)
         | SCall binds fname args =>
           bind_Some (params, rets, fbody) <- lookupFunction fname;
-            bind_Some argvs <- Common.option_all (List.map (interp_expr st) args);
-            bind_Some st0 <- Common.putmany params argvs Common.empty;
-            bind_Some (m', ob) <- interp_stmt f st0 m fbody;
+            bind_Some argvs <- Common.option_all (List.map (interp_expr l) args);
+            bind_Some l0 <- Common.putmany params argvs Map.empty_map;
+            bind_Some (m', ob) <- interp_stmt f m l0 fbody;
             match ob with
-            | inl (action, args, b) => Some (m', inl (action, args, BStack st b binds rets))
-            | inr st1 => 
-              bind_Some retvs <- Common.option_all (List.map (Common.get st1) rets);
-              bind_Some st' <- Common.putmany binds retvs st;
-              Some (m', inr st')
+            | inl (action, args, b) => Some (m', inl (action, args, BStack l b binds rets))
+            | inr l1 => 
+              bind_Some retvs <- Common.option_all (List.map (Map.get l1) rets);
+              bind_Some l' <- Common.putmany binds retvs l;
+              Some (m', inr l')
             end
         | SIO binds ionum args =>
-          bind_Some argvs <- Common.option_all (List.map (interp_expr st) args);
-          Some (m, inl (ionum, argvs, BWait st binds))
+          bind_Some argvs <- Common.option_all (List.map (interp_expr l) args);
+          Some (m, inl (ionum, argvs, BWait l binds))
         end
       end.
-    Definition exec_stmt st m c r := exists f, interp_stmt f st m c = Some r.
+    Definition exec_stmt m l c r := exists f, interp_stmt f m l c = Some r.
     
-    Fixpoint interp_cont(f: nat)(st: varmap)(m: mem)(c: cont): option computation_result :=
+    Fixpoint interp_cont(f: nat)(m: mem)(l: varmap)(c: cont): option computation_result :=
       match f with
       | 0 => None (* out of fuel *)
       | S f =>
         match c with
-        | (nil, c) => interp_stmt f st m c
-        | (cons (stf, binds, rets, cf) stack, c) =>
-          bind_Some (m', ob) <- interp_cont f stf m (stack, cf);
+        | (nil, c) => interp_stmt f m l c
+        | (cons (lf, binds, rets, cf) stack, c) =>
+          bind_Some (m', ob) <- interp_cont f m lf (stack, cf);
           match ob with
-          | inl (action, args, b) => Some (m', inl (action, args, BStack st b binds rets))
+          | inl (action, args, b) => Some (m', inl (action, args, BStack l b binds rets))
           | inr st1 => 
-            bind_Some retvs <- Common.option_all (List.map (Common.get st1) rets);
-            bind_Some st' <- Common.putmany binds retvs st;
-            interp_stmt f st' m' c
+            bind_Some retvs <- Common.option_all (List.map (Map.get st1) rets);
+            bind_Some l' <- Common.putmany binds retvs l;
+            interp_stmt f m' l' c
           end
         end
       end.
-    Definition exec_cont st m c r := exists f, interp_cont f st m c = Some r.
+    Definition exec_cont m l c r := exists f, interp_cont f m l c = Some r.
 
     (* If a predicate [P_x : forall b, Prop] identifies the return value of a partial function [f x],
        [arbitraryIfUndefined P_x] identifies the return value of [f x] when [f x] is defined and allows
@@ -155,14 +155,12 @@ Section Imp.
 
     Section WithWorld.
       Context {world : Type} (external_step : world -> mem*actname*list mword -> mem*list mword -> world -> Prop).
-      Definition interactive_step (s s' : world * computation_result) : Prop :=
+      (* Definition done (s : world * computation_result) : Prop :=  exists w m l, s = (w, (m, inr l)). *)
+      Definition step (s s' : world*computation_result) : Prop :=
         exists w m action argvs b, s = (w, (m, inl (action, argvs, b))) /\
         exists w' retvs m_, external_step w (m, action, argvs) (m_, retvs) w' /\
-        exists st' c', b retvs = Some (st', c') /\
-        exists m' R', exec_cont st' m_ c' (m', R') /\ s' = (w', (m', R')).
-      Definition done (s : world * computation_result) : Prop :=
-        exists w m l, s = (w, (m, inr l)).
-      Definition step s s' : Prop := not (done s) /\ arbitraryIfUndefined (interactive_step s) s'.
+        exists l' c', b retvs = Some (l', c') /\
+        exists m' R', arbitraryIfUndefined (exec_cont m_ l' c') (m', R') /\ s' = (w', (m', R')).
     End WithWorld.
 
     Section LabeledTransitionSystem.
@@ -173,3 +171,217 @@ Section Imp.
     End LabeledTransitionSystem.
   End WithFunctions.
 End Imp.
+
+
+
+
+
+Tactic Notation "texact" tactic(x) := exact x.
+Ltac head_of t :=
+  match t with
+  | ?t _ => head_of t
+  | _ => t
+  end.
+Notation "'subst!' y 'for' x 'in' f" := (match y with x => f end) (at level 10).
+Ltac beta1 x :=
+  lazymatch x with
+  | (fun a => ?f) ?b => constr:(subst! b for a in f)
+  end.
+Notation "'beta1!' x" := (ltac:(texact (beta1 x))) (only parsing, at level 10).
+
+Ltac apply_to_args_of f aapp :=
+  lazymatch aapp with
+  | (?g ?x) ?a => let r := apply_to_args_of f constr:(g x) in constr:(r a)
+  | _ ?a => constr:(f a)
+  | _ => f
+  end.
+
+Ltac induction_principle_definition T :=
+  let t := open_constr:(fun H:T => ltac:(induction H; exact I) : True) in
+  lazymatch open_constr:(fun H:T =>
+                           ltac:(let x := beta1 constr:(t H) in
+                                 let h := head_of x in exact h)
+                        ) with fun _ => ?v => v end.
+Ltac induction_principle_no_indices T :=
+  let T_ind := induction_principle_definition T in
+  let T_ind_args := apply_to_args_of T_ind T in
+  constr:(T_ind_args).
+Ltac is_indexed_inductive T :=
+  assert_succeeds(idtac; let h := head_of T in is_ind h);
+  assert_fails ltac:(idtac; let _ := induction_principle_no_indices T in idtac).
+
+(*
+Goal forall x y : nat, False. intros.
+  assert_succeeds (is_indexed_inductive (x = y)).
+  assert_fails (is_indexed_inductive nat).
+  assert_fails (is_indexed_inductive (prod nat nat)).
+  assert_fails (is_indexed_inductive (list nat)).
+*)
+
+
+
+
+
+Require Import Coq.Program.Equality.
+Module ht.
+  Section HoareLogic.
+    Goal True. let cls := constr:(ImpParameters) in match constr:(Set) with _ => (let none := constr:(_:cls) in idtac); fail 99 "DUPLICATE INSTANCE" | _ => idtac end. Abort.
+    Context {p : ImpParameters} (e : funname -> option (list varname * list varname * stmt)) {world : Type} (external_step : world -> mem*actname*list mword -> mem*list mword -> world -> Prop) (G : world -> mem -> Prop).
+
+    Inductive ht : (world -> mem -> varmap -> Prop) -> stmt -> (world -> mem -> varmap -> Prop) -> Prop :=
+    | set (P:_->_->_->Prop) x e (_:forall w m l, P w m l -> exists v, interp_expr l e = Some v)
+      : ht P (SSet x e) (fun w m l => exists l', P w m l' /\ exists v, interp_expr l' e = Some v /\ l = Map.put l' x v)
+    | skip P : ht P SSkip P
+    | io (P:_->_->_->Prop) binds action args
+         (_:forall w m l, P w m l ->
+                          exists argvs, Common.option_all (List.map (interp_expr l) args) = Some argvs /\
+                          forall m' retvs w', external_step w (m, action, argvs) (m', retvs) w' ->
+                                              G w' m' /\ exists l', Common.putmany binds retvs l = Some l')
+      : ht P (SIO binds action args) (fun w' m' l' =>  exists w m l argvs retvs,
+               P w m l /\ Common.option_all (List.map (interp_expr l) args) = Some argvs /\
+               external_step w (m, action, argvs) (m', retvs) w')
+    .
+    (* Notation "[ P ] c [ Q ]" := (ht P c Q) (at level 90, c at next level). *)
+
+    Inductive htc : (world -> mem -> varmap -> Prop) -> cont -> (world -> mem -> varmap -> Prop) -> Prop :=
+    | cskip P : htc P CSkip P
+    | cseq P c1 R (_:htc P c1 R) c2 Q (_:ht R c2 Q) : htc P (CSeq c1 c2) Q
+    | cweaken c (P Q P' Q':_->_->_->Prop) (_:htc P c Q) (_:forall w m l, P' w m l -> P w m l) (_:forall w m l, Q w m l -> Q' w m l) : htc P' c Q'
+      .
+
+    Lemma exec_cont_unique {m l c r1 r2} (_:exec_cont e m l c r1) (_:exec_cont e m l c r2) : r1 = r2.
+    Admitted.
+
+    Ltac t_step :=
+      match goal with
+      | _ => progress intros
+      | x:?T |- _ =>
+        assert_succeeds (let h := head_of T in is_ind h);
+        destruct x; []; (* TODO: use dependent elimination and allow indexed inductives *)
+        assert_fails (is_indexed_inductive T)
+      | H: ?x = ?y |- _ =>
+        let f := head_of x in
+        let g := head_of y in
+        is_constructor f; is_constructor g; inversion H;
+        subst; (* FIXME: only subst equations generated by inversion *)
+        clear H
+      end.
+    Ltac t := repeat t_step.
+    
+    Lemma ht_SSkip P Q (h : ht P SSkip Q) : forall w m l, P w m l -> Q w m l.
+    Proof. dependent induction h; eauto. Qed.
+
+    Lemma htc_SSkip P Q (h : htc P CSkip Q) : forall w m l, P w m l -> Q w m l.
+    Proof. dependent induction h; cbv [cont CSeq CSkip CStack] in *; t; eauto. Qed.
+
+    Definition invariant Q (s:world * computation_result) :=
+      let (w, result) := s in
+      match result with
+      | (m, (inl (action, args, blocked)))
+        => forall m' retvs w', external_step w (m, action, args) (m', retvs) w'
+                               -> exists l' c', blocked retvs = Some (l', c') /\ G w' m' /\ htc (fun w_ m_ l_ => w_ = w' /\ m_ = m' /\ l_ = l') c' Q
+      | (m, (inr l)) => Q w m l
+      end.
+
+    Lemma preservation P c Q (h : ht P c Q) w m l (HP: P w m l) :
+      exists r, exec_stmt e m l c r /\ invariant Q (w, r).
+    Proof with t.
+      dependent induction h; cbn in *.
+
+      { match goal with H:_ |- _ => pose proof (H _ _ _ ltac:(eauto)) end...
+        eexists.
+        split. { exists (S O). cbn. match goal with H:_ |- _ => rewrite H; reflexivity end. }
+        cbn. eauto. }
+      { eexists.
+        split. { exists (S O). cbn. reflexivity. }
+        cbn. eauto. }
+      { match goal with H:_ |- _ => pose proof (H _ _ _ ltac:(eauto)) end...
+        eexists.
+        unshelve (idtac; let e := open_constr:(_) in split; [apply e|pose proof e]).
+        { exists (S O). cbn. match goal with H:_ |- _ => rewrite H; reflexivity end. }
+        cbn.
+        intros.
+        match goal with H:_ |- _ => pose proof (H _ _ _ ltac:(eauto)) end...
+        eexists _, _.
+        cbv [BWait].
+        unshelve (idtac; let e := open_constr:(_) in split; [apply e|pose proof e]).
+        { match goal with H:_ |- _ => rewrite H; reflexivity end. }
+        intuition idtac.
+        eapply cweaken with (P := fun w_ m_ l_ => w_ = w' /\ m_ = m' /\ l_ = x0).
+        { econstructor. }
+        { eauto. }
+        cbn; intros.
+        repeat match goal with
+        | H:exists _, _ |- _ => destruct H
+        | H:_ /\ _ |- _ => destruct H
+        end.
+        subst.
+        eauto 9. }
+    Qed.
+
+    Lemma cpreservation P c Q (h : htc P c Q) w m l (HP: P w m l) :
+      exists r, exec_cont e m l c r /\ invariant Q (w, r).
+    Proof with t.
+      dependent induction h.
+      { eexists.
+        unshelve (idtac; let e := open_constr:(_) in split; [apply e|pose proof e]).
+        { exists (S (S O)). cbn. reflexivity. }
+        cbn; eauto. }
+      { match goal with H:_ |- _ => pose proof (H _ _ _ ltac:(eauto)) end...
+        destruct x as [?[?|?]].
+        { cbn in H1 |- *...
+          exists ((m0, inl (a, l0, BSeq b c2))).
+          split.
+          { admit. }
+          t.
+          match goal with H:_ |- _ => pose proof (H _ _ _ ltac:(eauto)) end...
+          eexists _, _.
+          split.
+          { cbv [BSeq]. match goal with H:_ |- _ => rewrite H; reflexivity end. }
+          intuition idtac.
+          eauto using cseq. }
+        { pose proof preservation _ _ _ H _ _ _ H1...
+          exists x.
+          split.
+          { admit. }
+          eauto. } }
+      { match goal with H:_ |- _ => pose proof (H _ _ _ ltac:(eauto)) end.
+        cbv [computation_result] in *... destruct s...
+        { eexists.
+          split; [solve[eauto]|].
+          cbn.
+          intros.
+          match goal with
+          | H:_ |- _ => pose proof (H _ _ _ ltac:(eauto))
+          end.
+          repeat match goal with
+                 | H:exists _, _ |- _ => destruct H
+                 | H:_ /\ _ |- _ => destruct H
+                 | H:_ * _ |- _ => destruct H
+                 end.
+          eexists _, _.
+          split.
+          eauto.
+          split.
+          eauto.
+          eapply cweaken.
+          eauto.
+          eauto.
+          eauto. }
+        { eexists.
+          split.
+          eauto.
+          cbn.
+          eauto. } }
+        Qed.
+
+    Lemma invariant_step Q s (HI:invariant Q s) s' (Hstep:step e external_step s s') : invariant Q s'.
+    Proof with t.
+      cbv [step] in *; destruct s as [? [?[?|?]]]...
+      match goal with H:_ |- _ => pose proof (H _ _ _ ltac:(eauto)) end...
+      assert (Some (x7, x8) = Some (x11, x12)) by congruence...
+      pose proof (cpreservation _ _ _ H4 _ _ _ ltac:(repeat constructor))...
+      specialize (H2 (ex_intro _ _ H5))...
+      match goal with H:_, G:_ |- _ => pose proof exec_cont_unique H G; clear G end; subst...
+      eauto. 
+    Qed.
